higher-order combinators for vldata, vllist

tests/layeff/LowParseWriters.Parsers.fst
@@ -159,6 +159,8 @@ let parse_vldata_intro_impl
     ICorrect () pos
   )
 
+let write_bounded_integer = LP.write_bounded_integer'
+
 let parse_vldata_intro_weak_impl
   #inv p min max
 = mk_repr_impl
